Further changes to Bezout proof

MotivatedMoves/AutoGeneralization/bezout.lean
@@ -7,8 +7,8 @@ open Autogeneralize Classical
 set_option trace.TypecheckingErrors true
 set_option trace.ProofPrinting true
 
-def is_gcd (g a b : ℤ) : Prop := g ∣ a ∧ g ∣ b ∧ (∀ c, c ∣ a → c ∣ b → c ∣ g)
-notation g " is GCD[" a ", " b "]" => is_gcd g a b
+def isGCD (g a b : ℤ) : Prop := g ∣ a ∧ g ∣ b ∧ (∀ c, c ∣ a → c ∣ b → c ∣ g)
+-- notation g " is GCD[" a ", " b "]" => isGCD g a b
 
 theorem Int.emod_natAbs_lt_of_nonzero (a : ℤ) {b : ℤ} (hbAbs : b.natAbs ≠ 0)  : (a % b).natAbs < b.natAbs := by
   have hb : b ≠ 0 := by exact natAbs_ne_zero.mp hbAbs
@@ -30,35 +30,36 @@ theorem Int.emod_natAbs_lt_of_nonzero (a : ℤ) {b : ℤ} (hbAbs : b.natAbs ≠ 
   exact emod_lt_of_pos a negb_pos
 
 /-- Bézout's identity states that for any two integers a and b, there exist integers x and y such that their greatest common divisor g can be expressed as a linear combination ax + by = g -/
-theorem bezout_identity (x y : ℤ) : x ≠ 0 → y ≠ 0 → ∃ (h k : ℤ), (h * x + k * y) is GCD[x, y] := by
-  intros _ y_neq_0
+theorem bezout_identity : ∀ (x y : ℤ), y ≠ 0 → ∃ (h k : ℤ), isGCD (h * x + k * y) x y := by
+  intros x y y_neq_0
 
   -- Consider the set A = {hx + ky | x,y ∈ ℤ}
   let A := {z : ℤ | ∃ h k : ℤ, z = h * x + k * y}
   -- Consider the set B = {|z| | z ∈ A, |z| ≠ 0} of non-zero absolute values
-  let B := (Int.natAbs '' A) \ {0}
-
   have A_add : ∀ a ∈ A, ∀ b ∈ A, a + b ∈ A := by
     rintro a ⟨h, k, a_eq⟩ b ⟨h', k', b_eq⟩
     use (h + h'), (k + k')
     rw [a_eq, b_eq]
-    rw [add_assoc, add_left_comm (k * y) _ _, ← add_assoc, ← add_mul, ← add_mul]
+    rw [add_assoc, Int.add_left_comm (k * y) _ _, ← add_assoc, ← add_mul, ← add_mul]
   have A_mul : ∀ a ∈ A, ∀ z : ℤ, z * a ∈ A := by
     rintro a ⟨h, k, a_eq⟩ z
     use z * h, z * k
     rw [a_eq]
     rw [mul_add, ← mul_assoc, ← mul_assoc]
 
+  let B := (Int.natAbs '' A) \ {0}
   -- Show B is non-empty by constructing an element
-  have hB_nonempty : B.Nonempty := by
+  have hB_nonempty : ∃ b : ℕ, b ∈ B := by
     use (0*x + 1*y).natAbs
-    refine ⟨⟨_, ⟨?elem_in_A, rfl⟩⟩, ?elem_abs_nonZero⟩
-    · use 0, 1
-    · rwa [Set.mem_singleton_iff, zero_mul, one_mul, zero_add, Int.natAbs_eq_zero]
-
+    change (0*x + 1*y).natAbs ∈ Int.natAbs '' A \ {0}
+    rw [@Set.mem_diff_singleton]
+    constructor
+    · apply Set.mem_image_of_mem Int.natAbs
+      use (discharger := rfl) 0, 1
+    · rwa [Int.zero_mul, Int.one_mul, Int.zero_add, @Ne.eq_def, Int.natAbs_eq_zero]
   -- By well-ordering principle on subsets of ℕ, B has a minimal element
   -- Call that minimal element "d"
-  -- let Bmin := Nat.find hB_nonempty
+  -- let Bmin : ℕ := @Nat.find B _ hB_nonempty
   obtain ⟨⟨d, (hdA : d ∈ A), (hdAbs_eq_Bmin : d.natAbs = _)⟩, (hBmin_neq_0 : _ ≠ 0)⟩ := Nat.find_spec hB_nonempty
   have hdAbs_neq_0 : d.natAbs ≠ 0 := by rwa [← hdAbs_eq_Bmin] at hBmin_neq_0
   have hd_min : ∀ z ∈ A, z.natAbs = 0 ∨ d.natAbs ≤ z.natAbs := by
@@ -93,9 +94,10 @@ theorem bezout_identity (x y : ℤ) : x ≠ 0 → y ≠ 0 → ∃ (h k : ℤ), (
       exact dvd_mul_left d q
     · rw [← Int.natAbs_eq_zero] at hr_eq_0
       have hd_min_r := hd_min r
-      contrapose hd_min_r
-      push_neg
-      refine' ⟨_, _, _⟩ <;> assumption
+      sorry
+      -- contrapose hd_min_r
+      -- push_neg
+      -- refine' ⟨_, _, _⟩ <;> assumption
 
   have hxA : x ∈ A := by use 1, 0; simp only [one_mul, zero_mul, add_zero]
   have d_dvd_x : d ∣ x := hd_div_A x hxA
@@ -112,8 +114,9 @@ theorem bezout_identity (x y : ℤ) : x ≠ 0 → y ≠ 0 → ∃ (h k : ℤ), (
     exact Dvd.dvd.linear_comb c_dvd_x c_dvd_y h k
 
 #print bezout_identity
+
 -- set_option maxHeartbeats 200000
--- set_option trace.AntiUnify true
+-- -- set_option trace.AntiUnify true
 example : True := by
   autogeneralize ℤ in bezout_identity
   trivial
